finish symbolic execution for sequential programs

ContractGeneration.thy
@@ -2,36 +2,59 @@ theory ContractGeneration
 imports Contracts
 begin
 
-fun map_of_eqs :: "form \<Rightarrow> (var \<Rightarrow> expr)" where
-  "map_of_eqs (f_eq (VarE v) e) = (VarE)(v:=e)"
-| "map_of_eqs ((f_eq (VarE v) e)\<^emph>f) = (map_of_eqs f)(v:=e)"
-| "map_of_eqs _ = VarE"
+fun map_of_eqs :: "form \<Rightarrow> (var \<rightharpoonup> expr)" where
+  "map_of_eqs ((f_eq (VarE v) e)\<^emph>f) = (map_of_eqs f)(v\<mapsto>e)"
+| "map_of_eqs _ = Map.empty"
+
+fun update_var_eq_after :: "form \<Rightarrow> (expr\<rightharpoonup>expr) \<Rightarrow> form" where
+  "update_var_eq_after (f_eq x y) arg_to_new_expr = 
+    (case arg_to_new_expr x of Some a \<Rightarrow> f_eq x a | None \<Rightarrow> f_eq x y)"
+| "update_var_eq_after ((f_eq x y)\<^emph>rest) arg_to_new_expr = 
+    ((case arg_to_new_expr x of Some a \<Rightarrow> f_eq x a | None \<Rightarrow> f_eq x y)
+    \<^emph>(update_var_eq_after rest arg_to_new_expr))"
+| "update_var_eq_after f _ = f"
+
+definition (in sound_separation_logic) bap :: "var set \<Rightarrow> var set \<Rightarrow> form \<Rightarrow> form \<Rightarrow> form \<Rightarrow> form \<Rightarrow> form \<Rightarrow> bool" where
+  "bap args Uq Qfree Qeq C M F \<equiv> entails (Qfree\<^emph>M) (add_prenex (sorted_list_of_set ((free_vars C \<union> free_vars F)
+    -(free_vars Qfree \<union> free_vars Qeq \<union> free_vars M))) (C\<^emph>F))
+  \<and> quantifree_symb_heap M \<and> quantifree_symb_heap F
+  \<and> free_vars M \<subseteq> UNIV - args - Uq \<and> free_vars F \<inter> args = {}"
 
 text \<open>As in 6.3.1 we assume a function body as a sequence of calls to functions for which we already 
   have the (conjunctive) contracts.\<close>
 locale generation_ctxt = program_logic +
   fixes func_body :: "(contract\<times>(var list)) list" and args :: "var list"
+  and bap_solver :: "var set \<Rightarrow> var set \<Rightarrow> form \<Rightarrow> form \<Rightarrow> form \<Rightarrow> (form\<times>form)"
   assumes non_empty: "func_body \<noteq> []" and conj: "list_all (conjunctive \<circ> fst) func_body"
-  and simple: "list_all (\<lambda>c. (\<exists>c'. fst (raw_contract (fst c)) = {c'})) func_body"
+  and simple: "list_all (\<lambda>c. (\<exists>c'. fst (raw_contract (fst c)) = [c'])) func_body"
   and well_formed: "list_all (\<lambda>c. set (snd c) \<subseteq> set (args) \<and> distinct (snd c)) func_body"
+  and bap_solution: "\<forall>uQ Qf Qeq C M F. bap_solver (set args) Uq Qf Qeq C = (M,F) 
+    \<longleftrightarrow> bap (set args) Uq Qf Qeq C M F"
 begin
 
-fun symbolic_execution :: "contract list \<Rightarrow> (form\<times>form) \<Rightarrow> (form\<times>form) option" where
-  "symbolic_execution [] (P,Q) = (P,Q)"
-  \<comment> \<open>TODO define actual symbolic execution step\<close>
+fun symbolic_execution :: "(contract\<times>(var list)) list \<Rightarrow> (form\<times>form) \<Rightarrow> (form\<times>form) option" where
+  "symbolic_execution [] (P,Q) = Some (P,Q)"
 | "symbolic_execution (func_call#rest) (P,Q) = 
-  (let _ = (case raw_contract func_call of (({(C,[D])},f),call_args) \<Rightarrow>
+  (case 
+    (case func_call of (contr, call_args) \<Rightarrow>
+    (case raw_contract contr of ([(C,[D])],f) \<Rightarrow>
     (case strip_prenex Q of (Uq, Qf\<^emph>Qeq) \<Rightarrow> 
     \<comment> \<open>Rename logical variables\<close>
-    (let (C1,vs) = rename_vars C (free_vars P - (set args)) id in
+    (let (C1,vs) = rename_vars C (free_vars P - (set args)) VarE in
     (let (D',_) = rename_vars D (free_vars P - (set (args))) vs in
+    (case strip_prenex D' of (_, Df\<^emph>Deq) \<Rightarrow> 
     \<comment> \<open>Substitute the arguments for the parameters\<close>
-    (let (C2,_) = rename_vars C1 {} (map_of (zip (snd f) call_args)) in
-    (let (C3,_) = rename_vars C2 {} (map_of_eqs Qeq) in
-    ())))))
-  | _ \<Rightarrow> None) in
-
-  symbolic_execution rest (P,Q))"
+    (let (C2,_) = rename_vars_option C1 {} ((map_of_eqs Qeq) \<circ>\<^sub>m (map_of (zip (snd f) call_args))) in
+    \<comment> \<open>Do biabduction and construct the next intermediate contract\<close>
+    (let (M,F) = bap_solver (set args) Uq Qf Qeq C2 in
+    (let P_after = M \<^emph> P in
+    (let Qf' = F \<^emph> Df in
+    (let Qeq' = update_var_eq_after Qeq ((map_of_eqs Deq) \<circ>\<^sub>m (map_of (zip (map VarE call_args) (snd f)))) in
+    (let Uq_after = (free_vars Qf' \<union> free_vars Qeq') - (set args) - free_vars P_after in
+    (let Q_after = add_prenex (sorted_list_of_set Uq_after) (Qf'\<^emph>Qeq') in
+    Some (P_after,Q_after))))))))
+  | _ \<Rightarrow> None))) | _ \<Rightarrow> None) | _ \<Rightarrow> None)) of Some (P_after,Q_after) \<Rightarrow>
+  symbolic_execution rest (P_after,Q_after) | _ \<Rightarrow> None)"
 
 fun build_initial :: "var list \<Rightarrow> var set \<Rightarrow> form" where
   "build_initial [] _ = Emp"
@@ -39,5 +62,10 @@ fun build_initial :: "var list \<Rightarrow> var set \<Rightarrow> form" where
 
 definition initialP :: form where
   "initialP \<equiv> simplify_emp_sepconj (build_initial args (set args))"
+
+text \<open>This is Theorem 3, but I won't prove it yet. This would be way to much work for now.\<close>
+lemma "symbolic_execution func_body (initialP, initialP) = Some (P,Q) \<Longrightarrow>
+  sound (Contract ([(P,[Q])], (f,args)))"
+  sorry
 end
 end
