Contracts.thy
@@ -6,6 +6,49 @@ fun strip_prenex :: "form \<Rightarrow> (var set \<times> form)" where
   "strip_prenex (Exists x f) = (let (vs,f') = strip_prenex f in (insert x vs,f'))"
 | "strip_prenex f = ({},f)"
 
+fun strip_prenexl :: "form \<Rightarrow> (var list \<times> form)" where
+  "strip_prenexl (Exists x f) = (let (vs,f') = strip_prenexl f in (x#vs,f'))"
+| "strip_prenexl f = ([],f)"
+
+lemma strip_set_list: "\<lbrakk>strip_prenex f = (vset,f'); strip_prenexl f = (vlist, f'')\<rbrakk>
+  \<Longrightarrow> vset = set vlist \<and> f'=f''"
+proof (induction f arbitrary: vset f' vlist f'')
+  case (Exists x1 f)
+  obtain vs2 f2 where step2: "strip_prenex f = (vs2,f2)" by fastforce
+  obtain vs3 f3 where step3: "strip_prenexl f = (vs3,f3)" by fastforce
+  have "strip_prenex (Exists x1 f) = (let (vs2,f2) = strip_prenex f in (insert x1 vs2,f2))" by simp
+  with step2 Exists(2) have first: "vset = insert x1 vs2" "f' = f2" by auto
+  have "strip_prenexl (Exists x1 f) = (let (vs2,f2) = strip_prenexl f in (x1#vs2,f2))" by simp
+  with step3 Exists(3) have "vlist = x1#vs3" "f'' = f3" by auto
+  with Exists(1)[OF step2 step3] first show ?case by auto
+qed (auto)
+
+fun add_prenex :: "var list \<Rightarrow> form \<Rightarrow> form" where
+  "add_prenex [] f = f"
+| "add_prenex (v#vs) f = Exists v (add_prenex vs f)"
+
+lemma strip_add_prenexl: 
+  "\<lbrakk>strip_prenexl (add_prenex vs f) = (vs',f'); strip_prenexl f = (vs'', f'')\<rbrakk>
+  \<Longrightarrow> vs'=vs@vs'' \<and> f'=f''"
+proof (induction vs arbitrary: f vs' f' vs'' f'')
+  case Nil
+  then show ?case by auto
+next
+  case (Cons a vs)
+  obtain vs2 f2 where IHaux: "strip_prenexl (add_prenex vs f) = (vs2,f2)" by fastforce
+  have "add_prenex (a#vs) f = (Exists a (add_prenex vs f))" by simp
+  then have "strip_prenexl (add_prenex (a#vs) f) = 
+    (let (vs2,f2) = strip_prenexl (add_prenex vs f) in (a#vs2,f2))" by simp
+  with IHaux Cons(2) have "vs' = a#vs2" "f'=f2" by auto
+  with Cons(1)[OF IHaux Cons(3)] have "vs' = a#vs@vs''" "f'=f''" by simp_all
+  then show ?case by simp
+qed
+
+lemma strip_add_prenex: 
+  "\<lbrakk>strip_prenex (add_prenex vs f) = (vs',f'); strip_prenex f = (vs'', f'')\<rbrakk>
+  \<Longrightarrow> vs'=set vs\<union>vs'' \<and> f'=f''"
+  using strip_add_prenexl strip_set_list by (metis set_append surj_pair)
+
 fun simplify_emp_sepconj :: "form \<Rightarrow> form" where
   "simplify_emp_sepconj (f1 \<^emph> f2) = 
   (case simplify_emp_sepconj f1 of Emp \<Rightarrow> simplify_emp_sepconj f2 
@@ -117,34 +160,32 @@ text \<open>The paper distinguishes program variables and logical variables.
   Therefore, we do not use different types for these two kinds of variables but just different sets.
   We also use meta-variables wherever possible.\<close>
  
-type_synonym pre_contract = "(form\<times>(form list)) set"
-
-value "simplify_emp_sepconj (foldr (\<lambda>(x,e) r. (f_eq x e) \<^emph> r) (zip [x,y] [X,Y]) Emp)"
+type_synonym pre_contract = "(form\<times>(form list)) list"
 
 typedef contract = "{(cs, (f,args))::pre_contract\<times>func | cs args f.
-  \<forall>(P,Q)\<in>cs. quantifier_free P \<and> symbolic_heap P \<and> \<comment> \<open>P is a quantifier-free symbolic heap\<close>
+  \<forall>(P,Q)\<in>set cs. quantifree_symb_heap P \<and> \<comment> \<open>P is a quantifier-free symbolic heap\<close>
   \<comment> \<open>Q is a disjunction of single formulas of the form \<open>\<exists>UQ. Qf \<^emph> Qeq\<close>\<close>
   list_all (\<lambda>q. case strip_prenex q of (UQ, Qf \<^emph> Qeq) \<Rightarrow>
     \<comment> \<open>The prenex variables are the logical ones in Qf and Qeq, that are not also in P.\<close>
     UQ = (free_vars Qf \<union> free_vars Qeq) - set args - free_vars P \<and>
     \<comment> \<open>Qf is a quantifier-free symbolic heap with only logical variables\<close>
-    quantifier_free Qf \<and> symbolic_heap Qf \<and> free_vars Qf \<inter> set args = {} \<and>
+    quantifree_symb_heap Qf \<and> free_vars Qf \<inter> set args = {} \<and>
     \<comment> \<open>Qeq is of the form \<open>x1=e1 \<^emph> ... \<^emph> xn=en \<^emph> Emp\<close> for arguments xi and some expressions e 
       that only contain logical variables.\<close>
     (\<exists>eqs. Qeq = simplify_emp_sepconj (foldr (\<lambda>(x, e). (\<^emph>) (f_eq x e)) (zip args eqs) Emp)
     \<and> list_all (\<lambda>e. free_vars e \<inter> set args = {}) eqs)
     | _ \<Rightarrow> False) Q \<and> Q \<noteq> []}" morphisms raw_contract Contract
-  by auto
+  by (smt (z3) empty_iff mem_Collect_eq set_empty2)
 
 setup_lifting type_definition_contract
 
 lift_definition conjunctive :: "contract \<Rightarrow> bool" is
-  "\<lambda>(cs, (f,args)). \<forall>(P,Qs) \<in> cs. length Qs = 1" .
+  "\<lambda>(cs, (f,args)). \<forall>(P,Qs) \<in> set cs. length Qs = 1" .
 
 context program_logic
 begin
 lift_definition sound :: "contract \<Rightarrow> bool" is
-  "\<lambda>(cs, (f,args)). \<forall>(P,Qs) \<in> cs. \<forall>c c' F.
+  "\<lambda>(cs, (f,args)). \<forall>(P,Qs) \<in> set cs. \<forall>c c' F.
     (((c \<turnstile> (P\<^emph>F)) \<and> fun_semantics fs f c c' \<and> symbolic_heap F \<and> free_vars F \<inter> set args = {}) 
     \<longrightarrow> (c' \<turnstile> ((star_disj Qs) \<^emph> F)))" .
 end
@@ -161,7 +202,7 @@ begin
 
 definition assign :: prog where "assign \<equiv> single_fun_prog (''assign'',[x,y]) (AssignVar x y)"
 definition assign_contract :: pre_contract where 
-  "assign_contract \<equiv> {(f_eq y Y,[Emp \<^emph> (f_eq x Y)\<^emph>(f_eq y Y)])}"
+  "assign_contract \<equiv> [(f_eq y Y,[Emp \<^emph> (f_eq x Y)\<^emph>(f_eq y Y)])]"
 lift_definition assign_c :: contract is "(assign_contract, (''assign'',[x,y]))"
 proof (auto simp: assign_contract_def)
   define eqs where "eqs = [VarE Y,VarE Y]"
@@ -174,7 +215,7 @@ qed
 
 definition const :: "val \<Rightarrow> prog" where "const k \<equiv> single_fun_prog (''const'',[x]) (AssignConst x k)"
 definition const_contract :: "val \<Rightarrow> pre_contract" where 
-  "const_contract k \<equiv> {(Emp,[Emp \<^emph> (f_eq x k)])}"
+  "const_contract k \<equiv> [(Emp,[Emp \<^emph> (f_eq x k)])]"
 lift_definition const_c :: "val \<Rightarrow> contract" is "\<lambda>k. (const_contract k, (''const'',[x]))"
 proof (auto simp: const_contract_def)
   fix k :: val
@@ -188,7 +229,7 @@ qed
 
 definition load :: prog where "load \<equiv> single_fun_prog (''load'',[x,y]) (Load x y)"
 definition load_contract :: pre_contract where 
-  "load_contract \<equiv> {((f_eq y Y)\<^emph>(Y\<mapsto>\<^sub>sz),[(Y\<mapsto>\<^sub>sz) \<^emph> (f_eq x z)\<^emph>(f_eq y Y)])}"
+  "load_contract \<equiv> [((f_eq y Y)\<^emph>(Y\<mapsto>\<^sub>sz),[(Y\<mapsto>\<^sub>sz) \<^emph> (f_eq x z)\<^emph>(f_eq y Y)])]"
 lift_definition load_c :: contract is "(load_contract, (''load'',[x,y]))"
   using var_sep[simplified]
 proof (auto simp: load_contract_def diff_var)
@@ -202,7 +243,7 @@ qed
 
 definition store :: prog where "store \<equiv> single_fun_prog (''store'',[x,y]) (Store x y)"
 definition store_contract :: pre_contract where 
-  "store_contract \<equiv> {((f_eq x X)\<^emph>(f_eq y Y)\<^emph>(X\<mapsto>\<^sub>sz),[(X\<mapsto>\<^sub>sY) \<^emph> (f_eq x X)\<^emph>(f_eq y Y)])}"
+  "store_contract \<equiv> [((f_eq x X)\<^emph>(f_eq y Y)\<^emph>(X\<mapsto>\<^sub>sz),[(X\<mapsto>\<^sub>sY) \<^emph> (f_eq x X)\<^emph>(f_eq y Y)])]"
 lift_definition store_c :: contract is "(store_contract, (''store'',[x,y]))"
   using var_sep[simplified]
 proof (auto simp: store_contract_def)
@@ -216,9 +257,9 @@ qed
 
 definition malloc :: prog where "malloc \<equiv> single_fun_prog (''malloc'',[x,y]) (Malloc x y)"
 definition malloc_contract :: pre_contract where 
-  "malloc_contract \<equiv> {((f_eq y Y),
+  "malloc_contract \<equiv> [((f_eq y Y),
     [Emp \<^emph> (f_eq x (null x))\<^emph>(f_eq y Y),
-    Exists u (((u\<mapsto>\<top>[Y])\<^emph>(f_eq (Base u) u)\<^emph>(f_eq (Ende u) (e_add u Y))) \<^emph> (f_eq x u)\<^emph>(f_eq y Y))])}"
+    Exists u (((u\<mapsto>\<top>[Y])\<^emph>(f_eq (Base u) u)\<^emph>(f_eq (Ende u) (e_add u Y))) \<^emph> (f_eq x u)\<^emph>(f_eq y Y))])]"
 lift_definition malloc_c :: contract is "(malloc_contract, (''malloc'',[x,y]))"
   using var_sep[simplified] diff_var
 proof (auto simp: malloc_contract_def)
@@ -239,9 +280,9 @@ qed
 
 definition free :: prog where "free \<equiv> single_fun_prog (''free'',[x]) (Free x)"
 definition free_contract :: pre_contract where 
-  "free_contract \<equiv> {
+  "free_contract \<equiv> [
   ((f_eq x X)\<^emph>(f_eq X null_loc), [(f_eq X null_loc) \<^emph> (f_eq x X)]),
-  ((f_eq x X)\<^emph>(X\<mapsto>\<top>[y])\<^emph>(f_eq (Base X) X)\<^emph>(f_eq (Ende X) (e_add X y)),[Emp \<^emph> (f_eq x X)])}"
+  ((f_eq x X)\<^emph>(X\<mapsto>\<top>[y])\<^emph>(f_eq (Base X) X)\<^emph>(f_eq (Ende X) (e_add X y)),[Emp \<^emph> (f_eq x X)])]"
 lift_definition free_c :: contract is "(free_contract, (''free'',[x]))"
   using var_sep[simplified]
 proof (auto simp: free_contract_def)
@@ -258,7 +299,7 @@ qed
 definition assign_binop :: "binop \<Rightarrow> prog" where "assign_binop op \<equiv> 
   single_fun_prog (''assign_binop'',[x,y,z]) (BinOp op x y z)"
 definition binop_contract :: "binop \<Rightarrow> pre_contract" where 
-  "binop_contract op \<equiv> {((f_eq y Y)\<^emph>(f_eq z Z),[Emp \<^emph> (f_eq x (BinOpE op Y Z))\<^emph>(f_eq y Y)\<^emph>(f_eq z Z)])}"
+  "binop_contract op \<equiv> [((f_eq y Y)\<^emph>(f_eq z Z),[Emp \<^emph> (f_eq x (BinOpE op Y Z))\<^emph>(f_eq y Y)\<^emph>(f_eq z Z)])]"
 lift_definition binop_c :: "binop \<Rightarrow> contract" is "\<lambda>op. (binop_contract op, (''assign_binop'',[x,y,z]))"
 proof (auto simp: binop_contract_def)
   fix op :: binop
@@ -273,7 +314,7 @@ qed
 definition assign_unop ::  "unop \<Rightarrow> prog" where "assign_unop op \<equiv> 
   single_fun_prog (''assign_unop'',[x,y]) (UnOp op x y)"
 definition unop_contract :: "unop \<Rightarrow> pre_contract" where 
-  "unop_contract op \<equiv> {((f_eq y Y),[Emp \<^emph> (f_eq x (UnOpE op Y))\<^emph>(f_eq y Y)])}"
+  "unop_contract op \<equiv> [((f_eq y Y),[Emp \<^emph> (f_eq x (UnOpE op Y))\<^emph>(f_eq y Y)])]"
 lift_definition unop_c :: "unop \<Rightarrow> contract" is "\<lambda>op. (unop_contract op, (''assign_unop'',[x,y]))"
 proof (auto simp: unop_contract_def)
   fix op :: unop
@@ -290,10 +331,9 @@ abbreviation "ptrplus\<phi> \<equiv> (Atom Neq (Base Y) null_loc)\<^emph>(f_eq (
   (f_eq (Ende Y) (Ende (e_add Y Z)))"
 abbreviation "ptrplus\<phi>2 \<equiv> (Atom Neq (Base Y) null_loc)\<^emph>(f_eq (e_add Y Z) (Ende Y))"
 definition ptrplus_contract :: pre_contract where 
-  "ptrplus_contract \<equiv> {
+  "ptrplus_contract \<equiv> [
   ((f_eq y Y)\<^emph>(f_eq z Z)\<^emph>ptrplus\<phi>,[ptrplus\<phi> \<^emph> (f_eq x (e_add Y Z))\<^emph>(f_eq y Y)\<^emph>(f_eq z Z)]),
-  ((f_eq y Y)\<^emph>(f_eq z Z)\<^emph>ptrplus\<phi>2,[ptrplus\<phi>2 \<^emph> (f_eq x (e_add Y Z))\<^emph>(f_eq y Y)\<^emph>(f_eq z Z)])
-  }"
+  ((f_eq y Y)\<^emph>(f_eq z Z)\<^emph>ptrplus\<phi>2,[ptrplus\<phi>2 \<^emph> (f_eq x (e_add Y Z))\<^emph>(f_eq y Y)\<^emph>(f_eq z Z)])]"
 lift_definition ptrplus_c :: contract is "(ptrplus_contract, (''ptrplus'',[x,y,z]))"
   using var_sep[simplified] diff_var
 proof (auto simp: ptrplus_contract_def)
@@ -310,8 +350,8 @@ qed
 
 definition ptrsub :: prog where "ptrsub \<equiv> single_fun_prog (''ptrsub'',[x,y,z]) (PtrSub x y z)"
 definition ptrsub_contract :: pre_contract where 
-  "ptrsub_contract \<equiv> {((f_eq y Y)\<^emph>(f_eq z Z)\<^emph>(Atom Neq (Base Y) null_loc)\<^emph>(Atom Leq (Base Y) Z)\<^emph>(Atom Leq Z (Ende Y)),
-  [Emp \<^emph> (f_eq x (BinOpE minus Y Z)\<^emph>(f_eq y Y)\<^emph>(f_eq z Z))])}"
+  "ptrsub_contract \<equiv> [((f_eq y Y)\<^emph>(f_eq z Z)\<^emph>(Atom Neq (Base Y) null_loc)\<^emph>(Atom Leq (Base Y) Z)\<^emph>(Atom Leq Z (Ende Y)),
+  [Emp \<^emph> (f_eq x (BinOpE minus Y Z)\<^emph>(f_eq y Y)\<^emph>(f_eq z Z))])]"
 lift_definition ptrsubs_c :: contract is "(ptrsub_contract, (''ptrsub'',[x,y,z]))"
 proof (auto simp: ptrsub_contract_def)
   fix op :: unop
@@ -329,13 +369,13 @@ text \<open>The contracts for assume and assert don't follow the scheme, as the 
   part of either Qf (it can't talk about program variables) or Qeq (it already contains all equalities.\<close>
 definition assume_f :: "condition \<Rightarrow> prog" where "assume_f c \<equiv> single_fun_prog (''assume'',[y,z]) (Assume c y z)"
 definition assume_contract :: "condition \<Rightarrow> pre_contract" where 
-  "assume_contract c \<equiv> {((f_eq y Y)\<^emph>(f_eq z Z),[Atom c y z \<^emph> (f_eq y Y)\<^emph>(f_eq z Z)])}"
+  "assume_contract c \<equiv> [((f_eq y Y)\<^emph>(f_eq z Z),[Atom c y z \<^emph> (f_eq y Y)\<^emph>(f_eq z Z)])]"
 lift_definition assume_c :: "condition \<Rightarrow> contract" is "\<lambda>c. (assume_contract c, (''assume'',[y,z]))"
   oops
 
 definition assert_f :: "condition \<Rightarrow> prog" where "assert_f c \<equiv> single_fun_prog (''assert'',[x,y]) (Assert c x y)"
 definition assert_contract :: "condition \<Rightarrow> pre_contract" where 
-  "assert_contract c \<equiv> {(Atom c y z\<^emph>(f_eq y Y)\<^emph>(f_eq z Z),[Atom c y z \<^emph> (f_eq y Y)\<^emph>(f_eq z Z)])}"
+  "assert_contract c \<equiv> [(Atom c y z\<^emph>(f_eq y Y)\<^emph>(f_eq z Z),[Atom c y z \<^emph> (f_eq y Y)\<^emph>(f_eq z Z)])]"
 lift_definition assert_c :: "condition \<Rightarrow> contract" is "\<lambda>c. (assert_contract c, (''assert'',[y,z]))"
   oops
 
